MECMAR/props/EarlyErrors.v
@@ -1,0 +1,99 @@
+From Warblre Require Import Base Patterns StaticSemantics.
+
+Module EarlyErrors.
+
+  Inductive SingletonCharacterEscape: CharacterEscape -> Character -> Prop :=
+  | Singleton_ctrl_t: SingletonCharacterEscape (CharacterEscape.ControlEsc ControlEscape.t) Characters.CHARACTER_TABULATION
+  | Singleton_ctrl_n: SingletonCharacterEscape (CharacterEscape.ControlEsc ControlEscape.n) Characters.LINE_FEED
+  | Singleton_ctrl_v: SingletonCharacterEscape (CharacterEscape.ControlEsc ControlEscape.v) Characters.LINE_TABULATION
+  | Singleton_ctrl_f: SingletonCharacterEscape (CharacterEscape.ControlEsc ControlEscape.f) Characters.FORM_FEED
+  | Singleton_ctrl_r: SingletonCharacterEscape (CharacterEscape.ControlEsc ControlEscape.r) Characters.CARRIAGE_RETURN
+  | Singleton_zero: SingletonCharacterEscape CharacterEscape.Zero Characters.NULL
+  | Singleton_id: forall c, SingletonCharacterEscape (CharacterEscape.IdentityEsc c) c.
+
+  Inductive SingletonClassAtom: ClassAtom -> Character -> Prop :=
+  | Singleton_SourceCharacter: forall c, SingletonClassAtom (SourceCharacter c) c
+  | Singleton_b: SingletonClassAtom (ClassEsc ClassEscape.b) Characters.BACKSPACE
+  | Singleton_dash: SingletonClassAtom (ClassEsc ClassEscape.Dash) Characters.HYPHEN_MINUS
+  | Singleton_char_esc: forall ce c,
+      SingletonCharacterEscape ce c -> SingletonClassAtom (ClassEsc (ClassEscape.CharacterEsc ce)) c.
+
+  Inductive ClassRanges: Patterns.ClassRanges -> Prop :=
+  | EmptyCR: ClassRanges Patterns.EmptyCR
+  | ClassAtomCR: forall ca t, ClassRanges t -> ClassRanges (Patterns.ClassAtomCR ca t)
+  | RangeCR: forall l h cl ch t,
+      SingletonClassAtom l cl ->
+      SingletonClassAtom h ch ->
+      (Character.numeric_value cl <= Character.numeric_value ch)%nat ->
+      ClassRanges t ->
+      ClassRanges (Patterns.RangeCR l h t).
+
+  Module Pass.
+    Inductive CharClass: Patterns.CharClass -> Prop :=
+    | NoninvertedCC: forall crs, ClassRanges crs -> CharClass (Patterns.NoninvertedCC crs)
+    | InvertedCC: forall crs, ClassRanges crs -> CharClass (Patterns.InvertedCC crs).
+
+    Inductive AtomEscape: Patterns.AtomEscape -> non_neg_integer -> Prop :=
+    | DecimalEsc: forall n m, (proj1_sig n) <= m -> AtomEscape (Patterns.AtomEscape.DecimalEsc n) m
+    | CharacterClassEsc: forall esc m, AtomEscape (Patterns.AtomEscape.CharacterClassEsc esc) m
+    | CharacterEsc: forall esc m, AtomEscape (Patterns.AtomEscape.CharacterEsc esc) m.
+
+    Inductive QuantifierPrefix: Patterns.QuantifierPrefix -> Prop :=
+    | Star: QuantifierPrefix Patterns.Star
+    | Plus: QuantifierPrefix Patterns.Plus
+    | Question: QuantifierPrefix Patterns.Question
+    | RepExact: forall n, QuantifierPrefix (Patterns.RepExact n)
+    | RepPartialRange: forall n, QuantifierPrefix (Patterns.RepPartialRange n)
+    | RepRange: forall min max, (min <= max)%nat -> QuantifierPrefix (Patterns.RepRange min max).
+
+    Inductive Quantifier: Patterns.Quantifier -> Prop :=
+    | Greedy: forall p, QuantifierPrefix p -> Quantifier (Patterns.Greedy p)
+    | Lazy: forall p, QuantifierPrefix p -> Quantifier (Patterns.Lazy p).
+
+    Inductive Regex: Patterns.Regex -> non_neg_integer -> Prop :=
+    | Empty: forall m, Regex Patterns.Empty m
+    | Char: forall chr m, Regex (Patterns.Char chr) m
+    | Dot: forall m, Regex Patterns.Dot m
+    | AtomEsc: forall esc m, AtomEscape esc m -> Regex (Patterns.AtomEsc esc) m
+    | CharacterClass: forall cc m, CharClass cc -> Regex (Patterns.CharacterClass cc) m
+    | Disjunction: forall r1 r2 m, Regex r1 m -> Regex r2 m -> Regex (Patterns.Disjunction r1 r2) m
+    | Quantified: forall r q m, Regex r m -> Quantifier q -> Regex (Patterns.Quantified r q) m
+    | Seq: forall r1 r2 m, Regex r1 m -> Regex r2 m -> Regex (Patterns.Seq r1 r2) m
+    | Group: forall name r m, Regex r m -> Regex (Patterns.Group name r) m
+    | Lookahead: forall r m, Regex r m -> Regex (Patterns.Lookahead r) m
+    | NegativeLookahead: forall r m, Regex r m -> Regex (Patterns.NegativeLookahead r) m
+    | Lookbehind: forall r m, Regex r m -> Regex (Patterns.Lookbehind r) m
+    | NegativeLookbehind: forall r m, Regex r m -> Regex (Patterns.NegativeLookbehind r) m.
+  End Pass.
+
+  Lemma countLeftCapturingParensBefore_contextualized: forall ctx f r m,
+      Root r f ctx ->
+      Pass.Regex r m ->
+      (countLeftCapturingParensBefore f ctx) + (countLeftCapturingParensWithin f ctx) <= m.
+    Proof. Admitted.
+      (* unfold Root.
+      induction ctx.
+      - intros f r n m Eq H. cbn in *. subst. unfold countLeftCapturingParensWithin.
+        destruct (existence f) as [ m' H' ].
+        apply shift_defs with (s := 1) in H'. cbn in *.
+        split.
+        + apply swap_refs with (1 := H') (2 := H).
+        + pose proof (unique_length_defs _ _ _ _ H) as <-. 
+          pose proof (monotony _ _ _ _ H).
+          lia.
+      - unfold countLeftCapturingParensBefore,countLeftCapturingParensWithin in *.
+        intros f r n m Eq H.
+        destruct a; cbn in Eq |- *;
+          specialize IHctx with (1 := Eq) (2 := H) as [ R B ]; cbn in R,B; dependent destruction R;
+          repeat match goal with | [ H: Ranges _ _ ?e _ |- _ ] => is_var e; pose proof (normalize_end_defs _ _ _ _ H) as -> end;
+          repeat rewrite -> Nat.add_0_r;
+          (* Normalize additions by first pushing + 1 to the right and then normalizing + nesting *)
+          repeat rewrite <- (Nat.add_assoc _ 1 _) in *;
+          repeat rewrite -> (Nat.add_comm 1 (countLeftCapturingParensWithin_impl _)) in *;
+          repeat rewrite -> Nat.add_assoc in *;
+          split; try (assumption + lia).
+        + rewrite <- Nat.add_1_r in R. apply shift_neg_defs with (s := 1) in R; try lia.
+          repeat rewrite -> Nat.add_sub in *.
+          apply shift_defs. assumption.
+    Qed. *)
+End EarlyErrors.
